programs/lean/Project.lean
@@ -1,3 +1,4 @@
+import Project.EncodeDecode.Spec
 import Project.NumInteger.Spec
 import Project.RustArray.Spec
 import Project.RustArrayTests.Spec
